src/proofs/no_slashable_attestations/supporting_lemmas/dv_next_preserves_ind_inv/ind_inv_dv_next.dfy
@@ -41,7 +41,7 @@ module Ind_Inv_DV_Next
     import opened Proofs_Intermediate_Steps
     
 
-    lemma lem_ind_inv_dv_next_invs_group_1(dv: DVState, e: DV.Event, dv': DVState)       
+    lemma lem_ind_inv_dv_next_invs_group_1(dv: DVState, e: DV.AttestationEvent, dv': DVState)       
     requires DV.NextEventPreCond(dv, e)
     requires DV.NextEvent(dv, e, dv')  
     requires ind_inv(dv)
@@ -54,7 +54,7 @@ module Ind_Inv_DV_Next
         lem_inv_latest_att_duty_is_rcvd_duty_dv_next(dv, e, dv');        
     }
 
-    lemma lem_ind_inv_dv_next_invs_group_2(dv: DVState, e: DV.Event, dv': DVState)       
+    lemma lem_ind_inv_dv_next_invs_group_2(dv: DVState, e: DV.AttestationEvent, dv': DVState)       
     requires DV.NextEventPreCond(dv, e)
     requires DV.NextEvent(dv, e, dv')  
     requires ind_inv(dv)
@@ -66,7 +66,7 @@ module Ind_Inv_DV_Next
         lem_inv_the_sequence_of_att_duties_is_in_order_of_slots_dv_next(dv, e, dv');                
     }
 
-    lemma lem_ind_inv_dv_next_invs_group_3(dv: DVState, e: DV.Event, dv': DVState)       
+    lemma lem_ind_inv_dv_next_invs_group_3(dv: DVState, e: DV.AttestationEvent, dv': DVState)       
     requires DV.NextEventPreCond(dv, e)
     requires DV.NextEvent(dv, e, dv')  
     requires ind_inv(dv)
@@ -77,7 +77,7 @@ module Ind_Inv_DV_Next
         lem_inv_no_active_consensus_instances_before_the_first_att_duty_was_received_dv_next(dv, e, dv');                        
     }
 
-    lemma lem_ind_inv_dv_next_invs_group_4(dv: DVState, e: DV.Event, dv': DVState)       
+    lemma lem_ind_inv_dv_next_invs_group_4(dv: DVState, e: DV.AttestationEvent, dv': DVState)       
     requires DV.NextEventPreCond(dv, e)
     requires DV.NextEvent(dv, e, dv')  
     requires ind_inv(dv)
@@ -90,7 +90,7 @@ module Ind_Inv_DV_Next
         lem_inv_rcvd_att_duties_are_from_dv_seq_of_att_duties_dv_next(dv, e, dv');    
     }
 
-    lemma lem_ind_inv_dv_next_invs_group_5(dv: DVState, e: DV.Event, dv': DVState)       
+    lemma lem_ind_inv_dv_next_invs_group_5(dv: DVState, e: DV.AttestationEvent, dv': DVState)       
     requires DV.NextEventPreCond(dv, e)
     requires DV.NextEvent(dv, e, dv')  
     requires ind_inv(dv)
@@ -101,7 +101,7 @@ module Ind_Inv_DV_Next
         lem_inv_current_validity_predicate_for_slot_k_is_stored_in_att_slashing_db_hist_k_dv_next(dv, e, dv');          
     }
 
-    lemma lem_ind_inv_dv_next_invs_group_6(dv: DVState, e: DV.Event, dv': DVState)       
+    lemma lem_ind_inv_dv_next_invs_group_6(dv: DVState, e: DV.AttestationEvent, dv': DVState)       
     requires DV.NextEventPreCond(dv, e)
     requires DV.NextEvent(dv, e, dv')  
     requires ind_inv(dv)
@@ -112,7 +112,7 @@ module Ind_Inv_DV_Next
         lem_inv_construct_signed_attestation_signature_assumptions_helper_dv_next(dv, e, dv');  
     }
 
-    lemma lem_ind_inv_dv_next_invs_group_7(dv: DVState, e: DV.Event, dv': DVState)       
+    lemma lem_ind_inv_dv_next_invs_group_7(dv: DVState, e: DV.AttestationEvent, dv': DVState)       
     requires DV.NextEventPreCond(dv, e)
     requires DV.NextEvent(dv, e, dv')  
     requires ind_inv(dv)
@@ -200,7 +200,7 @@ module Ind_Inv_DV_Next
         lem_inv_data_of_all_created_attestations_is_a_set_of_decided_values_dv_next(dv);
     }
    
-    lemma lem_ind_inv_dv_next_inv_all_validity_predicates_are_stored_in_att_slashing_db_hist(dv: DVState, e: DV.Event, dv': DVState)  
+    lemma lem_ind_inv_dv_next_inv_all_validity_predicates_are_stored_in_att_slashing_db_hist(dv: DVState, e: DV.AttestationEvent, dv': DVState)  
     requires DV.NextEventPreCond(dv, e)
     requires DV.NextEvent(dv, e, dv')       
     requires ind_inv(dv)
@@ -229,7 +229,7 @@ module Ind_Inv_DV_Next
         assert inv_all_validity_predicates_are_stored_in_att_slashing_db_hist(dv');
     }
 
-    lemma lem_ind_inv_dv_next_inv_exists_an_honest_node_that_sent_an_att_share_for_every_submitted_att(dv: DVState, e: DV.Event, dv': DVState)       
+    lemma lem_ind_inv_dv_next_inv_exists_an_honest_node_that_sent_an_att_share_for_every_submitted_att(dv: DVState, e: DV.AttestationEvent, dv': DVState)       
     requires DV.NextEventPreCond(dv, e)
     requires DV.NextEvent(dv, e, dv')  
     requires ind_inv(dv)
@@ -265,7 +265,7 @@ module Ind_Inv_DV_Next
         assert inv_exists_an_honest_node_that_sent_an_att_share_for_every_submitted_att(dv');
     }
 
-    lemma lem_ind_inv_dv_next_inv_decided_values_of_consensus_instances_are_decided_by_a_quorum(dv: DVState, e: DV.Event, dv': DVState)       
+    lemma lem_ind_inv_dv_next_inv_decided_values_of_consensus_instances_are_decided_by_a_quorum(dv: DVState, e: DV.AttestationEvent, dv': DVState)       
     requires DV.NextEventPreCond(dv, e)
     requires DV.NextEvent(dv, e, dv')  
     requires ind_inv(dv)
@@ -274,7 +274,7 @@ module Ind_Inv_DV_Next
         lem_inv_decided_values_of_consensus_instances_are_decided_by_a_quorum(dv, e, dv');
     }
 
-    lemma lem_ind_inv_dv_next_inv_every_sent_validity_predicate_is_based_on_a_rcvd_att_duty_and_a_slashing_db_for_dv(dv: DVState, e: DV.Event, dv': DVState)       
+    lemma lem_ind_inv_dv_next_inv_every_sent_validity_predicate_is_based_on_a_rcvd_att_duty_and_a_slashing_db_for_dv(dv: DVState, e: DV.AttestationEvent, dv': DVState)       
     requires DV.NextEventPreCond(dv, e)
     requires DV.NextEvent(dv, e, dv')  
     requires ind_inv(dv)
@@ -283,7 +283,7 @@ module Ind_Inv_DV_Next
         lem_inv_every_sent_validity_predicate_is_based_on_a_rcvd_att_duty_and_a_slashing_db_for_dv_next(dv, e, dv');
     }
 
-    lemma lem_ind_inv_dv_next_inv_every_sent_validity_predicate_is_based_on_a_rcvd_att_duty_and_a_slashing_db(dv: DVState, e: DV.Event, dv': DVState)       
+    lemma lem_ind_inv_dv_next_inv_every_sent_validity_predicate_is_based_on_a_rcvd_att_duty_and_a_slashing_db(dv: DVState, e: DV.AttestationEvent, dv': DVState)       
     requires DV.NextEventPreCond(dv, e)
     requires DV.NextEvent(dv, e, dv')  
     requires ind_inv(dv)
@@ -292,7 +292,7 @@ module Ind_Inv_DV_Next
         lem_inv_every_sent_validity_predicate_is_based_on_a_rcvd_att_duty_and_a_slashing_db(dv, e, dv');
     }
 
-    lemma lem_ind_inv_dv_next_inv_a_decided_value_of_a_consensus_instance_for_slot_k_is_for_slot_k(dv: DVState, e: DV.Event, dv': DVState)       
+    lemma lem_ind_inv_dv_next_inv_a_decided_value_of_a_consensus_instance_for_slot_k_is_for_slot_k(dv: DVState, e: DV.AttestationEvent, dv': DVState)       
     requires DV.NextEventPreCond(dv, e)
     requires DV.NextEvent(dv, e, dv')  
     requires ind_inv(dv)
@@ -302,7 +302,7 @@ module Ind_Inv_DV_Next
     }
 
     
-    lemma lem_ind_inv_dv_next_invs_group_8(dv: DVState, e: DV.Event, dv': DVState)       
+    lemma lem_ind_inv_dv_next_invs_group_8(dv: DVState, e: DV.AttestationEvent, dv': DVState)       
     requires DV.NextEventPreCond(dv, e)
     requires DV.NextEvent(dv, e, dv')  
     requires ind_inv(dv)
@@ -315,7 +315,7 @@ module Ind_Inv_DV_Next
         lem_ind_inv_dv_next_inv_every_sent_validity_predicate_is_based_on_a_rcvd_att_duty_and_a_slashing_db(dv, e, dv');   
     }
 
-    lemma lem_ind_inv_dv_next_inv_in_transit_messages_are_in_allMessagesSent(dv: DVState, e: DV.Event, dv': DVState)       
+    lemma lem_ind_inv_dv_next_inv_in_transit_messages_are_in_allMessagesSent(dv: DVState, e: DV.AttestationEvent, dv': DVState)       
     requires DV.NextEventPreCond(dv, e)
     requires DV.NextEvent(dv, e, dv')  
     requires ind_inv(dv)
@@ -325,7 +325,7 @@ module Ind_Inv_DV_Next
         lem_inv_all_in_transit_messages_were_sent_inv_in_transit_messages_are_in_allMessagesSent(dv');
     }
 
-    lemma lem_ind_inv_dv_next_inv_38(dv: DVState, e: DV.Event, dv': DVState)       
+    lemma lem_ind_inv_dv_next_inv_38(dv: DVState, e: DV.AttestationEvent, dv': DVState)       
     requires DV.NextEventPreCond(dv, e)
     requires DV.NextEvent(dv, e, dv')  
     requires ind_inv(dv)
@@ -336,7 +336,7 @@ module Ind_Inv_DV_Next
         lem_inv_attestation_shares_to_broadcast_are_sent_messages_dv_next(dv, e, dv');
     }
 
-    lemma lem_ind_inv_dv_next_inv_exists_att_duty_in_dv_seq_of_att_duty_for_every_slot_in_att_slashing_db_hist(dv: DVState, e: DV.Event, dv': DVState)       
+    lemma lem_ind_inv_dv_next_inv_exists_att_duty_in_dv_seq_of_att_duty_for_every_slot_in_att_slashing_db_hist(dv: DVState, e: DV.AttestationEvent, dv': DVState)       
     requires DV.NextEventPreCond(dv, e)
     requires DV.NextEvent(dv, e, dv')  
     requires ind_inv(dv)
@@ -345,7 +345,7 @@ module Ind_Inv_DV_Next
         lem_inv_exists_att_duty_in_dv_seq_of_att_duty_for_every_slot_in_att_slashing_db_hist(dv, e, dv');
     }
 
-    lemma lem_ind_inv_dv_next_invs_group_9(dv: DVState, e: DV.Event, dv': DVState)       
+    lemma lem_ind_inv_dv_next_invs_group_9(dv: DVState, e: DV.AttestationEvent, dv': DVState)       
     requires DV.NextEventPreCond(dv, e)
     requires DV.NextEvent(dv, e, dv')  
     requires ind_inv(dv)
@@ -357,7 +357,7 @@ module Ind_Inv_DV_Next
         lem_inv_attestation_shares_to_broadcast_are_sent_messages_inv_attestation_shares_to_broadcast_is_a_subset_of_all_messages_sent(dv');
     }
 
-    lemma lem_ind_inv_dv_next_invs_group_10(dv: DVState, e: DV.Event, dv': DVState)       
+    lemma lem_ind_inv_dv_next_invs_group_10(dv: DVState, e: DV.AttestationEvent, dv': DVState)       
     requires DV.NextEventPreCond(dv, e)
     requires DV.NextEvent(dv, e, dv')  
     requires ind_inv(dv)
@@ -370,7 +370,7 @@ module Ind_Inv_DV_Next
         lem_inv_data_of_att_shares_are_decided_values_dv_next(dv, e, dv');
     }
     
-    lemma lem_ind_inv_dv_next_inv_future_decisions_known_by_dvc_are_decisions_of_quorums(dv: DVState, e: DV.Event, dv': DVState)       
+    lemma lem_ind_inv_dv_next_inv_future_decisions_known_by_dvc_are_decisions_of_quorums(dv: DVState, e: DV.AttestationEvent, dv': DVState)       
     requires DV.NextEventPreCond(dv, e)
     requires DV.NextEvent(dv, e, dv')  
     requires ind_inv(dv)
@@ -381,7 +381,7 @@ module Ind_Inv_DV_Next
         lem_inv_future_decisions_known_by_dvc_are_decisions_of_quorums(dv, e, dv');
     }
 
-    lemma lem_ind_inv_dv_next_inv_slots_in_future_decided_data_are_correct(dv: DVState, e: DV.Event, dv': DVState)       
+    lemma lem_ind_inv_dv_next_inv_slots_in_future_decided_data_are_correct(dv: DVState, e: DV.AttestationEvent, dv': DVState)       
     requires DV.NextEventPreCond(dv, e)
     requires DV.NextEvent(dv, e, dv')  
     requires ind_inv(dv)
@@ -391,7 +391,7 @@ module Ind_Inv_DV_Next
         lem_inv_slots_in_future_decided_data_are_correct(dv, e, dv');
     }
 
-    lemma lem_ind_inv_dv_next_invs_group_11(dv: DVState, e: DV.Event, dv': DVState)       
+    lemma lem_ind_inv_dv_next_invs_group_11(dv: DVState, e: DV.AttestationEvent, dv': DVState)       
     requires DV.NextEventPreCond(dv, e)
     requires DV.NextEvent(dv, e, dv')  
     requires ind_inv(dv)
@@ -402,7 +402,7 @@ module Ind_Inv_DV_Next
         lem_inv_slots_in_future_decided_data_are_correct(dv, e, dv');        
     }
 
-    lemma lem_ind_inv_dv_next_invs_group_12(dv: DVState, e: DV.Event, dv': DVState)       
+    lemma lem_ind_inv_dv_next_invs_group_12(dv: DVState, e: DV.AttestationEvent, dv': DVState)       
     requires DV.NextEventPreCond(dv, e)
     requires DV.NextEvent(dv, e, dv')  
     requires ind_inv(dv)
@@ -417,7 +417,7 @@ module Ind_Inv_DV_Next
         lem_inv_no_rcvd_att_duties_are_higher_than_latest_att_duty_dv_next(dv, e, dv');  
     }
 
-    lemma lem_ind_inv_dv_next_invs_group_13(dv: DVState, e: DV.Event, dv': DVState)       
+    lemma lem_ind_inv_dv_next_invs_group_13(dv: DVState, e: DV.AttestationEvent, dv': DVState)       
     requires DV.NextEventPreCond(dv, e)
     requires DV.NextEvent(dv, e, dv')  
     requires ind_inv(dv)
@@ -429,7 +429,7 @@ module Ind_Inv_DV_Next
         lem_inv_unchanged_dvc_rs_pubkey_dv_next(dv, e, dv');
     }
 
-    lemma lem_ind_inv_dv_next_invs_group_14(dv: DVState, e: DV.Event, dv': DVState)       
+    lemma lem_ind_inv_dv_next_invs_group_14(dv: DVState, e: DV.AttestationEvent, dv': DVState)       
     requires DV.NextEventPreCond(dv, e)
     requires DV.NextEvent(dv, e, dv')  
     requires ind_inv(dv)
@@ -444,7 +444,7 @@ module Ind_Inv_DV_Next
         lem_inv_db_of_vp_contains_all_data_of_sent_att_shares_with_lower_slots_dv_next(dv, e, dv');        
     }
     
-    lemma lem_ind_inv_dv_next_ind_inv_helper_1(dv: DVState, e: DV.Event, dv': DVState)       
+    lemma lem_ind_inv_dv_next_ind_inv_helper_1(dv: DVState, e: DV.AttestationEvent, dv': DVState)       
     requires DV.NextEventPreCond(dv, e)
     requires DV.NextEvent(dv, e, dv')  
     requires ind_inv(dv)
@@ -457,7 +457,7 @@ module Ind_Inv_DV_Next
         lem_ind_inv_dv_next_invs_group_3(dv, e, dv');
     }
 
-    lemma lem_ind_inv_dv_next_ind_inv_helper_2(dv: DVState, e: DV.Event, dv': DVState)  
+    lemma lem_ind_inv_dv_next_ind_inv_helper_2(dv: DVState, e: DV.AttestationEvent, dv': DVState)  
     requires DV.NextEventPreCond(dv, e)
     requires DV.NextEvent(dv, e, dv')  
     requires ind_inv(dv)    
@@ -474,7 +474,7 @@ module Ind_Inv_DV_Next
         lem_ind_inv_dv_next_invs_group_8(dv, e, dv');
     }
 
-    lemma lem_ind_inv_dv_next_ind_inv_helper_3(dv: DVState, e: DV.Event, dv': DVState)       
+    lemma lem_ind_inv_dv_next_ind_inv_helper_3(dv: DVState, e: DV.AttestationEvent, dv': DVState)       
     requires DV.NextEventPreCond(dv, e)
     requires DV.NextEvent(dv, e, dv')  
     requires ind_inv(dv)
@@ -487,7 +487,7 @@ module Ind_Inv_DV_Next
         lem_ind_inv_dv_next_invs_group_11(dv, e, dv');                                     
     }
 
-    lemma lem_ind_inv_dv_next_ind_inv_helper_4(dv: DVState, e: DV.Event, dv': DVState)       
+    lemma lem_ind_inv_dv_next_ind_inv_helper_4(dv: DVState, e: DV.AttestationEvent, dv': DVState)       
     requires DV.NextEventPreCond(dv, e)
     requires DV.NextEvent(dv, e, dv')  
     requires ind_inv(dv)
@@ -500,7 +500,7 @@ module Ind_Inv_DV_Next
         lem_ind_inv_dv_next_invs_group_14(dv, e, dv');                              
     }
 
-    lemma lem_ind_inv_dv_next_ind_inv_helper_a(dv: DVState, e: DV.Event, dv': DVState)       
+    lemma lem_ind_inv_dv_next_ind_inv_helper_a(dv: DVState, e: DV.AttestationEvent, dv': DVState)       
     requires DV.NextEventPreCond(dv, e)
     requires DV.NextEvent(dv, e, dv')  
     requires ind_inv(dv) 
@@ -517,7 +517,7 @@ module Ind_Inv_DV_Next
         lem_ind_inv_dv_next_ind_inv_helper_2(dv, e, dv');    
     }
 
-    lemma lem_ind_inv_dv_next_ind_inv_helper_b(dv: DVState, e: DV.Event, dv': DVState)       
+    lemma lem_ind_inv_dv_next_ind_inv_helper_b(dv: DVState, e: DV.AttestationEvent, dv': DVState)       
     requires DV.NextEventPreCond(dv, e)
     requires DV.NextEvent(dv, e, dv')  
     requires ind_inv(dv) 
@@ -532,7 +532,7 @@ module Ind_Inv_DV_Next
         lem_ind_inv_dv_next_ind_inv_helper_4(dv, e, dv');    
     }
 
-    lemma lem_ind_inv_dv_next_ind_inv_helper(dv: DVState, e: DV.Event, dv': DVState)       
+    lemma lem_ind_inv_dv_next_ind_inv_helper(dv: DVState, e: DV.AttestationEvent, dv': DVState)       
     requires DV.NextEventPreCond(dv, e)
     requires DV.NextEvent(dv, e, dv')  
     requires ind_inv(dv) 
@@ -555,7 +555,7 @@ module Ind_Inv_DV_Next
         lem_ind_inv_dv_next_ind_inv_helper_b(dv, e, dv');                
     }
 
-    lemma lem_ind_inv_dv_next_ind_inv(dv: DVState, e: DV.Event, dv': DVState)       
+    lemma lem_ind_inv_dv_next_ind_inv(dv: DVState, e: DV.AttestationEvent, dv': DVState)       
     requires DV.NextEventPreCond(dv, e)
     requires DV.NextEvent(dv, e, dv')  
     requires ind_inv(dv)    
