src/proofs/no_slashable_attestations/supporting_lemmas/dv_next_preserves_ind_inv/invs_dv_next_1.dfy
@@ -24,21 +24,21 @@ module Invs_DV_Next_1
     import opened Fnc_Invs_1
     import opened Helper_Sets_Lemmas
 
-    lemma lem_inv_all_honest_nodes_is_a_quorum_dv_next(dv: DVState, event: DV.Event, dv': DVState)       
+    lemma lem_inv_all_honest_nodes_is_a_quorum_dv_next(dv: DVState, event: DV.AttestationEvent, dv': DVState)       
     requires NextEventPreCond(dv, event)
     requires NextEvent(dv, event, dv')  
     requires inv_all_honest_nodes_is_a_quorum(dv)
     ensures inv_all_honest_nodes_is_a_quorum(dv')
     { }    
 
-    lemma lem_inv_unchanged_paras_of_consensus_instances_dv_next(dv: DVState, event: DV.Event, dv': DVState)       
+    lemma lem_inv_unchanged_paras_of_consensus_instances_dv_next(dv: DVState, event: DV.AttestationEvent, dv': DVState)       
     requires NextEventPreCond(dv, event)
     requires NextEvent(dv, event, dv')  
     requires inv_unchanged_paras_of_consensus_instances(dv)
     ensures inv_unchanged_paras_of_consensus_instances(dv')
     { }    
 
-    lemma lem_inv_only_dv_construct_signed_attestation_signature_dv_next(dv: DVState, event: DV.Event, dv': DVState)       
+    lemma lem_inv_only_dv_construct_signed_attestation_signature_dv_next(dv: DVState, event: DV.AttestationEvent, dv': DVState)       
     requires NextEventPreCond(dv, event)
     requires NextEvent(dv, event, dv')  
     requires inv_only_dv_construct_signed_attestation_signature(dv)
@@ -49,7 +49,7 @@ module Invs_DV_Next_1
 
     lemma lem_inv_current_att_duty_is_rcvd_duty_dv_next(
         dv: DVState,
-        event: DV.Event,
+        event: DV.AttestationEvent,
         dv': DVState
     )    
     requires NextEventPreCond(dv, event)
@@ -93,7 +93,7 @@ module Invs_DV_Next_1
 
     lemma lem_inv_latest_att_duty_is_rcvd_duty_dv_next(
         dv: DVState,
-        event: DV.Event,
+        event: DV.AttestationEvent,
         dv': DVState
     )    
     requires NextEventPreCond(dv, event)
@@ -137,7 +137,7 @@ module Invs_DV_Next_1
 
     lemma lem_inv_none_latest_att_duty_implies_none_current_att_duty_dv_next(
         dv: DVState,
-        event: DV.Event,
+        event: DV.AttestationEvent,
         dv': DVState
     )    
     requires NextEventPreCond(dv, event)
@@ -185,7 +185,7 @@ module Invs_DV_Next_1
 
     lemma lem_inv_current_att_duty_is_either_none_or_latest_att_duty_dv_next(
         dv: DVState,
-        event: DV.Event,
+        event: DV.AttestationEvent,
         dv': DVState
     )    
     requires NextEventPreCond(dv, event)
@@ -233,7 +233,7 @@ module Invs_DV_Next_1
 
     lemma lem_inv_available_current_att_duty_is_latest_att_duty_dv_next(
         dv: DVState,
-        event: DV.Event,
+        event: DV.AttestationEvent,
         dv': DVState
     )    
     requires NextEventPreCond(dv, event)
@@ -282,7 +282,7 @@ module Invs_DV_Next_1
     
     lemma lem_inv_the_sequence_of_att_duties_is_in_order_of_slots_dv_next(
         dv: DVState,
-        event: DV.Event,
+        event: DV.AttestationEvent,
         dv': DVState
     )    
     requires NextEventPreCond(dv, event)
@@ -296,7 +296,7 @@ module Invs_DV_Next_1
 
     lemma lem_inv_no_duplicated_att_duties_dv_next(
         dv: DVState,
-        event: DV.Event,
+        event: DV.AttestationEvent,
         dv': DVState
     )    
     requires NextEventPreCond(dv, event)
@@ -307,7 +307,7 @@ module Invs_DV_Next_1
 
     lemma lem_pred_unchanged_dvn_seq_of_att_duties_dv_next(
         dv: DVState,
-        event: DV.Event,
+        event: DV.AttestationEvent,
         dv': DVState
     )    
     requires NextEventPreCond(dv, event)
@@ -317,7 +317,7 @@ module Invs_DV_Next_1
 
     lemma lem_inv_every_att_duty_before_dvn_att_index_was_delivered_f_serve_attestation_duty(
         dv: DVState,
-        event: DV.Event,
+        event: DV.AttestationEvent,
         dv': DVState
     )  
     requires inv_all_honest_nodes_is_a_quorum(dv)    
@@ -404,7 +404,7 @@ module Invs_DV_Next_1
 
     lemma lem_inv_every_att_duty_before_dvn_att_index_was_delivered_dv_next(
         dv: DVState,
-        event: DV.Event,
+        event: DV.AttestationEvent,
         dv': DVState
     )
     requires inv_all_honest_nodes_is_a_quorum(dv)    
@@ -452,7 +452,7 @@ module Invs_DV_Next_1
     
     lemma lem_inv_no_active_consensus_instances_before_the_first_att_duty_was_received_dv_next(
         dv: DVState,
-        event: DV.Event,
+        event: DV.AttestationEvent,
         dv': DVState
     )    
     requires NextEventPreCond(dv, event)
@@ -500,7 +500,7 @@ module Invs_DV_Next_1
 
     lemma lem_inv_slots_of_active_consensus_instances_are_not_higher_than_the_slot_of_latest_att_duty_dv_next(
         dv: DVState,
-        event: DV.Event,
+        event: DV.AttestationEvent,
         dv': DVState
     )    
     requires NextEventPreCond(dv, event)
@@ -564,7 +564,7 @@ module Invs_DV_Next_1
     
     lemma lem_inv_dvc_has_a_corresponding_att_duty_for_every_active_attestation_consensus_instance_dv_next(
         dv: DVState,
-        event: DV.Event,
+        event: DV.AttestationEvent,
         dv': DVState
     )    
     requires NextEventPreCond(dv, event)
@@ -616,7 +616,7 @@ module Invs_DV_Next_1
 
     lemma lem_inv_the_consensus_instance_indexed_k_is_for_the_rcvd_duty_at_slot_k_dv_next(
         dv: DVState,
-        event: DV.Event,
+        event: DV.AttestationEvent,
         dv': DVState
     )    
     requires NextEventPreCond(dv, event)
