src/proofs/no_slashable_attestations/supporting_lemmas/dv_next_preserves_ind_inv/invs_dv_next_3.dfy
@@ -33,7 +33,7 @@ module Invs_DV_Next_3
 
     lemma lem_inv_att_slashing_db_hist_keeps_track_only_of_rcvd_att_duties_dv_next(
         dv: DVState,
-        event: DV.Event,
+        event: DV.AttestationEvent,
         dv': DVState
     )    
     requires NextEventPreCond(dv, event)
@@ -84,7 +84,7 @@ module Invs_DV_Next_3
 
     lemma lem_inv_exist_a_db_in_att_slashing_db_hist_and_an_att_duty_for_every_validity_predicate_dv_next(
         dv: DVState,
-        event: DV.Event,
+        event: DV.AttestationEvent,
         dv': DVState
     )    
     requires NextEventPreCond(dv, event)
@@ -136,7 +136,7 @@ module Invs_DV_Next_3
 
     lemma lem_inv_current_validity_predicate_for_slot_k_is_stored_in_att_slashing_db_hist_k_dv_next(
         dv: DVState,
-        event: DV.Event,
+        event: DV.AttestationEvent,
         dv': DVState
     )    
     requires NextEventPreCond(dv, event)
@@ -188,7 +188,7 @@ module Invs_DV_Next_3
 
     lemma lem_inv_monotonic_att_slashing_db_dv_next(
         dv: DVState,
-        event: DV.Event,
+        event: DV.AttestationEvent,
         dv': DVState
     )    
     requires NextEventPreCond(dv, event)
@@ -235,7 +235,7 @@ module Invs_DV_Next_3
 
     lemma lem_inv_every_db_in_att_slashing_db_hist_is_a_subset_of_att_slashing_db_dv_next(
         dv: DVState,
-        event: DV.Event,
+        event: DV.AttestationEvent,
         dv': DVState
     )    
     requires NextEventPreCond(dv, event)
@@ -287,7 +287,7 @@ module Invs_DV_Next_3
 
     lemma lem_inv_monotonic_att_slashing_db_hist_dv_next(
         dv: DVState,
-        event: DV.Event,
+        event: DV.AttestationEvent,
         dv': DVState
     )    
     requires NextEventPreCond(dv, event)
@@ -334,7 +334,7 @@ module Invs_DV_Next_3
 
     lemma lem_inv_active_att_consensus_instances_are_tracked_in_att_slashing_db_hist_dv_next(
         dv: DVState,
-        event: DV.Event,
+        event: DV.AttestationEvent,
         dv': DVState
     )    
     requires NextEventPreCond(dv, event)
@@ -382,7 +382,7 @@ module Invs_DV_Next_3
 
     lemma lem_inv_construct_signed_attestation_signature_assumptions_helper_dv_next(
         dv: DVState,
-        event: DV.Event,
+        event: DV.AttestationEvent,
         dv': DVState
     )    
     requires NextEventPreCond(dv, event)
@@ -408,7 +408,7 @@ module Invs_DV_Next_3
     
     lemma lem_inv_all_in_transit_messages_were_sent_dv_next(
         dv: DVState,
-        event: DV.Event,
+        event: DV.AttestationEvent,
         dv': DVState
     )    
     requires NextEventPreCond(dv, event)
@@ -442,10 +442,10 @@ module Invs_DV_Next_3
 
     lemma lem_inv_attestation_shares_to_broadcast_are_sent_messages_HonestNodeTakingStep(
         dv: DVState,
-        event: DV.Event,
+        event: DV.AttestationEvent,
         dv': DVState,
         node: BLSPubkey, 
-        nodeEvent: Types.Event, 
+        nodeEvent: Types.AttestationEvent, 
         nodeOutputs: Outputs
     )       
     requires NextEventPreCond(dv, event)
@@ -553,7 +553,7 @@ module Invs_DV_Next_3
 
     lemma lem_inv_attestation_shares_to_broadcast_are_sent_messages_dv_next(
         dv: DVState,
-        event: DV.Event,
+        event: DV.AttestationEvent,
         dv': DVState
     )       
     requires NextEventPreCond(dv, event)
@@ -584,10 +584,10 @@ module Invs_DV_Next_3
 
     lemma lem_inv_rcvd_att_shares_are_from_sent_messages_ReceivedAttestationShare(
         dv: DVState,
-        event: DV.Event,
+        event: DV.AttestationEvent,
         dv': DVState,
         node: BLSPubkey, 
-        nodeEvent: Types.Event, 
+        nodeEvent: Types.AttestationEvent, 
         nodeOutputs: Outputs,
         attestation_share: AttestationShare
     )       
@@ -714,7 +714,7 @@ module Invs_DV_Next_3
 
     lemma lem_inv_rcvd_att_shares_are_from_sent_messages_dv_next(
         dv: DVState,
-        event: DV.Event,
+        event: DV.AttestationEvent,
         dv': DVState
     )       
     requires NextEventPreCond(dv, event)
@@ -766,7 +766,7 @@ module Invs_DV_Next_3
 
     lemma lem_inv_available_latest_att_duty_is_from_dv_seq_of_att_duties_new_body_dv_next(
         dv: DVState,
-        event: DV.Event,
+        event: DV.AttestationEvent,
         dv': DVState
     )    
     requires NextEvent.requires(dv, event, dv')  
@@ -783,7 +783,7 @@ module Invs_DV_Next_3
 
     lemma lem_inv_rcvd_att_duties_are_from_dv_seq_of_att_duties_dv_next(
         dv: DVState,
-        event: DV.Event,
+        event: DV.AttestationEvent,
         dv': DVState
     )    
     requires NextEventPreCond(dv, event)
@@ -871,7 +871,7 @@ module Invs_DV_Next_3
 
     lemma lem_inv_none_latest_att_duty_and_empty_set_of_rcvd_att_duties_dv_next(
         dv: DVState,
-        event: DV.Event,
+        event: DV.AttestationEvent,
         dv': DVState
     )    
     requires NextEventPreCond(dv, event)
@@ -922,7 +922,7 @@ module Invs_DV_Next_3
 
     lemma lem_inv_no_rcvd_att_duties_are_higher_than_latest_att_duty_dv_next(
         dv: DVState,
-        event: DV.Event,
+        event: DV.AttestationEvent,
         dv': DVState
     )    
     requires NextEventPreCond(dv, event)
@@ -974,10 +974,10 @@ module Invs_DV_Next_3
 
     lemma lem_inv_unique_rcvd_att_duty_per_slot_dv_next_HonestNodeTakingStep(
         dv: DVState,
-        event: DV.Event,
+        event: DV.AttestationEvent,
         dv': DVState,
         node: BLSPubkey, 
-        nodeEvent: Types.Event, 
+        nodeEvent: Types.AttestationEvent, 
         nodeOutputs: Outputs,
         attestation_duty: AttestationDuty
     )    
@@ -1019,7 +1019,7 @@ module Invs_DV_Next_3
 
     lemma lem_inv_unique_rcvd_att_duty_per_slot_dv_next(
         dv: DVState,
-        event: DV.Event,
+        event: DV.AttestationEvent,
         dv': DVState
     )    
     requires NextEventPreCond(dv, event)
